step 2: refactor 3d options

src/3d/Options.fst
@@ -7,124 +7,317 @@ module OS = OS
 
 #push-options "--warn_error -272" //top-level effects are okay
 
-let arg0 : ref string = alloc "3d"
+inline_for_extraction
+let valid_string
+  (valid: (string -> Tot bool))
+: Tot Type0
+= (s: string { valid s == true })
+
+let always_valid (_: string) : Tot bool = true
+
+inline_for_extraction
+let vstring = valid_string always_valid
+
+(* NOTE: default arguments here MUST be set to "", false, [] or None *)
+
+let arg0 : ref vstring = alloc ""
 let batch : ref bool = alloc false
-let check_hashes : ref (option check_hashes_t) = alloc None
 let clang_format : ref bool = alloc false
-let clang_format_executable : ref string = alloc ""
+let clang_format_executable : ref vstring = alloc ""
 let cleanup : ref bool = alloc false
 let debug : ref bool = alloc false
-let error_log : ref (option string) = alloc None
-let error_log_function : ref (option string) = alloc None
-let inplace_hashes : ref (list string) = alloc []
+let error_log : ref (option vstring) = alloc None
+let error_log_function : ref (option vstring) = alloc None
+let inplace_hashes : ref (list vstring) = alloc []
 let input_file : ref (list string) = alloc []
-let module_name : ref (option string) = alloc None
-let no_everparse_h : ref bool = alloc false
-let output_dir : ref (option string) = alloc None
+let no_copy_everparse_h : ref bool = alloc false
+let output_dir : ref vstring = alloc ""
 let save_hashes : ref bool = alloc false
 let skip_makefiles : ref bool = alloc false
 
-let set_check_hashes = function
-| "none" -> check_hashes := None
-| "weak" -> batch := true; check_hashes := Some WeakHashes
-| "strong" -> batch := true; check_hashes := Some StrongHashes
-| "inplace" -> batch := true; check_hashes := Some InplaceHashes
-| _ -> ()
-
-let equate_types_list : ref (list (string & string)) = alloc []
-
-(* We would like to parse --help as an option, but this would
-   require to recurse on the definition of the list of options. To
-   avoid that, we define this list as mutable, and then we add --help
-   after the fact. *)
-
-let options0 =
-  let open FStar.Getopt in
-  [
-   (noshort, "batch", ZeroArgs (fun _ -> batch := true), "Verify the generated F* code and extract C code");
-   (noshort, "check_hashes", OneArg (set_check_hashes, "none|weak|strong"), "Check hashes");
-   (noshort, "check_inplace_hash", OneArg ((fun c -> inplace_hashes := c :: !inplace_hashes), "file.3d=file.h"), "Check hashes stored in one .h/.c file");
-   (noshort, "clang_format", ZeroArgs (fun _ -> batch := true; clang_format := true), "Call clang-format on extracted .c/.h files (--batch only)");
-   (noshort, "clang_format_executable", OneArg ((fun cmd -> batch := true; clang_format := true; clang_format_executable := cmd), "clang-format full path"), "Provide path to clang-format if not reachable through PATH");
-   (noshort, "cleanup", ZeroArgs (fun _ -> cleanup := true), "Remove *.fst*, *.krml and kremlin-args.rsp (--batch only)");
-   (noshort, "copy_everparse_h", ZeroArgs (fun _ -> no_everparse_h := false), "Copy EverParse.h (--batch only)");
-   (noshort, "debug", ZeroArgs (fun _ -> debug := true), "Emit a lot of debugging output");
-   (noshort, "error_log", OneArg ((fun l -> error_log := Some l), "error log"), "The stream to which to log errors (default 'stderr')");
-   (noshort, "error_log_function", OneArg ((fun l -> error_log_function := Some l), "error logging function"), "The function to use to log errors  (default 'fprintf')");
-   (noshort, "no_batch", ZeroArgs (fun _ -> batch := false), "Do not verify the generated F* code or extract C code");
-   (noshort, "no_clang_format", ZeroArgs (fun _ -> clang_format := false), "Do not call clang-format on extracted .c/.h files");
-   (noshort, "no_cleanup", ZeroArgs (fun _ -> cleanup := false), "Do not remove *.fst*, *.krml or kremlin-args.rsp");
-   (noshort, "no_copy_everparse_h", ZeroArgs (fun _ -> no_everparse_h := true), "Do not copy EverParse.h");
-   (noshort, "no_save_hashes", ZeroArgs (fun _ -> save_hashes := false), "Do not save hashes");
-   (noshort, "no_skip_makefiles", ZeroArgs (fun _ -> skip_makefiles := false), "Generate Makefile.basic, Makefile.include (--batch only)");
-   (noshort, "odir", OneArg ((fun dir -> output_dir := Some dir), "output directory"), "output directory (default '.'); writes <module_name>.fst and <module_name>_wrapper.c to the output directory");
-   (noshort, "save_hashes", ZeroArgs (fun _ -> save_hashes := true), "Save hashes");
-   (noshort, "skip_makefiles", ZeroArgs (fun _ -> skip_makefiles := true), "Do not generate Makefile.basic, Makefile.include");
-   (noshort, "version", ZeroArgs (fun _ -> FStar.IO.print_string (Printf.sprintf "EverParse/3d %s\nCopyright 2018, 2019, 2020 Microsoft Corporation\n" Version.everparse_version); exit 0), "Show this version of EverParse");
-   (noshort, "module_name", OneArg ((fun mname -> module_name := Some mname), "module name"), "module name to use for the output file");
-   (noshort, "equate_types", OneArg ((fun str ->
+let valid_equate_types (str: string) : Tot bool =
      let l = String.split [','] str in
      match l with
-     | [m1;m2] -> equate_types_list := (m1, m2)::(!equate_types_list)
-     | _ -> failwith (Printf.sprintf "Bad argument to equate_types %s\n" str)), "A, B"), "Takes an argument of the form A,B and then for each entrypoint definition in B, it generates an assert (A.t == B.t) in the B.Types file, useful when refactoring specs, you can provide multiple equate_types on the command line");
-   ]
+     | [m1;m2] -> true
+     | _ -> false
 
-let options : ref _ = alloc options0
+let equate_types_list : ref (list (valid_string valid_equate_types)) = alloc []
 
-let display_usage () : ML unit =
+let valid_check_hashes : string -> Tot bool = function
+| "weak"
+| "strong"
+| "inplace"
+  -> true
+| _ -> false
+
+let check_hashes : ref (option (valid_string valid_check_hashes)) = alloc None
+
+noeq
+type cmd_option_kind =
+  | OptBool:
+      (v: ref bool) ->
+      cmd_option_kind
+  | OptString:
+      (arg_desc: string) ->
+      (valid: (string -> Tot bool)) ->
+      (v: ref (valid_string valid)) ->
+      cmd_option_kind
+  | OptStringOption:
+      (arg_desc: string) ->
+      (valid: (string -> Tot bool)) ->
+      (v: ref (option (valid_string valid))) ->
+      cmd_option_kind
+  | OptList:
+      (arg_desc: string) ->
+      (valid: (string -> Tot bool)) ->
+      (v: ref (list (valid_string valid))) ->
+      cmd_option_kind
+
+noeq
+type cmd_option
+= | CmdOption:
+    (name: string) ->
+    (kind: cmd_option_kind) ->
+    (desc: string) ->
+    (implies: list string) (* name of OptBool to set to true *) ->
+    cmd_option
+  | CmdFStarOption of FStar.Getopt.opt
+
+let cmd_option_name (a: cmd_option) : Tot string =
+  match a with
+  | CmdFStarOption (_, name', _, _)
+  | CmdOption name' _ _ _
+    -> name'
+
+let rec find_cmd_option (name: string) (l: list cmd_option): Tot (option cmd_option) = match l with
+  | [] -> None
+  | a :: q ->
+    if name = cmd_option_name a then Some a else find_cmd_option name q
+
+let cmd_option_description (a: cmd_option) : Tot string =
+  match a with
+  | CmdOption _ _ desc _
+  | CmdFStarOption (_, _, _, desc) ->
+    desc
+
+let cmd_option_arg_desc (a: cmd_option) : Tot string =
+  match a with
+  | CmdFStarOption (_, _, arg, _) ->
+    begin match arg with
+    | FStar.Getopt.OneArg (_, argdesc) -> argdesc
+    | _ -> ""
+    end
+  | CmdOption _ kind _ _ ->
+    begin match kind with
+    | OptString argdesc _ _
+    | OptStringOption argdesc _ _
+    | OptList argdesc _ _
+      -> argdesc
+    | _ -> ""
+    end
+
+let cmd_option_has_negation (a: cmd_option) : Tot bool =
+  match a with
+  | CmdOption _ k _ _ ->
+    OptBool? k || OptStringOption? k
+  | _ -> false
+
+let set_implies (options: ref (list cmd_option)) (implies: list string) : ML unit =
+  List.iter
+    (fun name ->
+      match find_cmd_option name !options with
+      | Some (CmdOption _ (OptBool x) _ _) -> x := true
+      | _ -> ()
+    )
+    implies
+
+let string_starts_with (big small: string) : Tot bool =
+  let small_len = String.length small in
+  if String.length big < small_len
+  then false
+  else String.sub big 0 small_len = small
+
+let negate_string_gen (s: string) (negation: string) =
+  if s `string_starts_with` negation
+  then String.sub s (String.length negation) (String.length s - String.length negation)
+  else negation ^ s
+
+let name_is_negated (s: string) : Tot bool = s `string_starts_with` "no_"
+let negate_name (s: string) : Tot string = negate_string_gen s "no_"
+let negate_description (s: string) : Tot string = negate_string_gen s "Do not"
+
+let fstar_options_of_cmd_option
+  (options: ref (list cmd_option))
+  (o: cmd_option)
+: Tot (list FStar.Getopt.opt)
+= match o with
+  | CmdFStarOption f -> [f]
+  | CmdOption name kind desc implies ->
+    begin match kind with
+    | OptBool v ->
+      [
+        (FStar.Getopt.noshort, name, FStar.Getopt.ZeroArgs (fun _ -> set_implies options implies; v := true), desc);
+        (FStar.Getopt.noshort, negate_name name, FStar.Getopt.ZeroArgs (fun _ -> v := false), negate_description desc);
+      ]
+    | OptString arg_desc valid v ->
+      [(
+        FStar.Getopt.noshort, name,
+        FStar.Getopt.OneArg (
+          (fun (x: string) ->
+             if valid x
+             then begin
+               set_implies options implies;
+               v := x
+             end else
+               failwith (Printf.sprintf "Bad argument to %s: got %s, expected %s" name x arg_desc)
+          ),
+          arg_desc
+        ),
+        desc
+      )]
+    | OptStringOption arg_desc valid v ->
+      [
+        (
+          FStar.Getopt.noshort, name,
+          FStar.Getopt.OneArg (
+            (fun (x: string) ->
+              if valid x
+              then begin
+                set_implies options implies;
+                v := Some x
+              end else
+                failwith (Printf.sprintf "Bad argument to %s: got %s, expected %s" name x arg_desc)
+            ),
+            arg_desc
+          ),
+          desc
+        );
+        (FStar.Getopt.noshort, negate_name name, FStar.Getopt.ZeroArgs (fun _ -> v := None), negate_description desc)
+      ]
+    | OptList arg_desc valid v ->
+      [(
+        FStar.Getopt.noshort, name,
+        FStar.Getopt.OneArg (
+          (fun (x: string) ->
+            if valid x
+            then begin
+              set_implies options implies;
+              v := x :: !v
+            end else
+              failwith (Printf.sprintf "Bad argument to %s: got %s, expected %s" name x arg_desc)
+          ),
+          arg_desc
+        ),
+        desc
+      )]
+    end
+
+let compute_current_options (options: ref (list cmd_option)) : ML string =
+  (* we need to accumulate those boolean options implied by other options but that might be manually toggled by the user,
+     but without duplicates
+   *)
+  let update_manually_untoggled_1 (mu: list string) (opt: string) : ML (list string) =
+    match find_cmd_option opt !options with
+    | Some (CmdOption _ (OptBool v) _ _) ->
+      if !v then mu else if List.Tot.mem opt mu then mu else opt :: mu
+    | _ -> mu
+  in
+  let update_manually_untoggled (mu: list string) (s: list string) : ML (list string) =
+    List.fold_left update_manually_untoggled_1 mu s
+  in
+  (* first print the values of current options *)
+  let print (msg_mu: string & list string) (opt: cmd_option) : ML (string & list string) =
+    match opt with
+    | CmdOption name kind desc implies ->
+      let (msg, mu) = msg_mu in
+      begin match kind with
+      | OptBool v ->
+        if !v
+        then (Printf.sprintf "%s --%s" msg name, update_manually_untoggled mu implies)
+        else msg_mu
+      | OptString _ _ v ->
+        let v = !v in
+        if v = ""
+        then msg_mu
+        else (Printf.sprintf "%s --%s %s" msg name v, update_manually_untoggled mu implies)
+      | OptStringOption _ _ v ->
+        begin match !v with
+        | None -> msg_mu
+        | Some v -> (Printf.sprintf "%s --%s %s" msg name v, update_manually_untoggled mu implies)
+        end
+      | OptList _ _ v ->
+        let v = !v in
+        if Nil? v
+        then msg_mu
+        else
+          let app (msg: string) (s: string) = Printf.sprintf "%s --%s %s" msg name s in
+          (List.Tot.fold_left app msg (List.Tot.rev v) (* list was accumulated as a fifo *),
+            update_manually_untoggled mu implies)
+      end
+    | _ -> msg_mu
+  in
+  let (msg, manually_untoggled) = List.fold_left print ("", []) !options in
+  (* then print the untoggling of those options manually toggled by the user *)
+  let print_untoggle (msg: string) (opt: string) : Tot string =
+    Printf.sprintf "%s --%s" msg (negate_name opt)
+  in
+  let msg = List.Tot.fold_left print_untoggle msg manually_untoggled in
+  (* finally, append the input files *)
+  let app (msg: string) (s: string) : Tot string = Printf.sprintf "%s %s" msg s in
+  List.Tot.fold_left app msg !input_file
+
+let display_usage_1 (options: ref (list cmd_option)) : ML unit =
   FStar.IO.print_string "EverParse/3d: verified data validation with dependent data descriptions\n";
   FStar.IO.print_string "\n";
-  FStar.IO.print_string (Printf.sprintf "Usage: %s [options] path_to_input_file1.3d path_to_input_file2.3d ... \n" !arg0);
+  FStar.IO.print_string (Printf.sprintf "Usage: %s [options] path_to_input_file1.3d path_to_input_file2.3d ... \n" (if !arg0 = "" then "3d" else !arg0));
   FStar.IO.print_string "\n";
   FStar.IO.print_string "Options:\n";
-  List.iter (fun (_, m, arg, desc) ->
-    let argdesc = match arg with
-    | FStar.Getopt.OneArg (_, argdesc) -> Printf.sprintf " <%s>" argdesc
-    | _ -> ""
-    in
-    FStar.IO.print_string (Printf.sprintf "--%s%s\n\t%s\n" m argdesc desc))
+  List.iter
+    (fun x ->
+      let m = cmd_option_name x in
+      let desc = cmd_option_description x in
+      let argdesc = cmd_option_arg_desc x in
+      let argdesc = if argdesc = "" then "" else Printf.sprintf "<%s>" argdesc in
+      let visible = not (m `string_starts_with` "__") in
+      let negate = if cmd_option_has_negation x then Printf.sprintf " (opposite is --%s)" (negate_name m) else "" in
+      if visible then FStar.IO.print_string (Printf.sprintf "--%s%s%s\n\t%s\n" m argdesc negate desc)
+    )
     !options
-      ;
-  FStar.IO.print_string "\n";
-  if !batch then begin
-    FStar.IO.print_string "--batch is currently toggled.\n";
-    if !clang_format then begin
-      FStar.IO.print_string "--clang_format is currently toggled.\n"
-    end;
-    if !cleanup then begin
-      FStar.IO.print_string "--cleanup is currently toggled.\n"
-    end;
-    if !skip_makefiles then begin
-      FStar.IO.print_string "--skip_makefiles is currently toggled.\n"
-    end;
-    if not !no_everparse_h then begin
-      FStar.IO.print_string "--copy_everparse_h is currently toggled.\n"
-    end;
-    let chk = match !check_hashes with
-    | None -> "none"
-    | Some WeakHashes -> "weak"
-    | Some StrongHashes -> "strong"
-    | Some InplaceHashes -> "inplace"
-    in
-    FStar.IO.print_string (Printf.sprintf "--check_hashes is currently set to %s.\n" chk);
-    if !save_hashes then begin
-      FStar.IO.print_string "--save_hashes is currently toggled.\n"
-    end;
-    ()
-  end
+    ;
+  FStar.IO.print_string (Printf.sprintf "\nCurrent options are:%s\n" (compute_current_options options))
 
-let _ =
-  options := ('h', "help", FStar.Getopt.ZeroArgs (fun _ -> display_usage (); exit 0), "Show this help message") :: !options
+let (display_usage_2, fstar_options) =
+  let options : ref (list cmd_option) = alloc [] in
+  let display_usage () = display_usage_1 options in
+  options := [
+    CmdOption "batch" (OptBool batch) "Verify the generated F* code and extract C code" [];
+    CmdOption "check_hashes" (OptStringOption "weak|strong|inplace" valid_check_hashes check_hashes) "Check hashes" ["batch"];
+    CmdOption "check_inplace_hash" (OptList "file.3d=file.h" always_valid inplace_hashes) "Check hashes stored in one .h/.c file" [];
+    CmdOption "clang_format" (OptBool clang_format) "Call clang-format on extracted .c/.h files (--batch only)" ["batch"];
+    CmdOption "clang_format_executable" (OptString "clang-format full path" always_valid clang_format_executable) "Set the path to clang-format if not reachable through PATH" ["batch"; "clang_format"];
+    CmdOption "cleanup" (OptBool cleanup) "Remove *.fst*, *.krml and kremlin-args.rsp (--batch only)" [];
+    CmdOption "no_copy_everparse_h" (OptBool no_copy_everparse_h) "Do not Copy EverParse.h (--batch only)" [];
+    CmdOption "debug" (OptBool debug) "Emit a lot of debugging output" [];
+    CmdOption "error_log" (OptStringOption "error log" always_valid error_log) "Set the stream to which to log errors (default 'stderr')" [];
+    CmdOption "error_log_function" (OptStringOption "error logging function" always_valid error_log_function) "Use a function to log errors (default 'fprintf')" [];
+    CmdFStarOption ('h', "help", FStar.Getopt.ZeroArgs (fun _ -> display_usage (); exit 0), "Show this help message");
+    CmdOption "odir" (OptString "output directory" always_valid output_dir) "output directory (default '.'); writes <module_name>.fst and <module_name>_wrapper.c to the output directory" [];
+    CmdOption "save_hashes" (OptBool save_hashes) "Save hashes" [];
+    CmdOption "skip_makefiles" (OptBool skip_makefiles) "Do not Generate Makefile.basic, Makefile.include" [];
+    CmdFStarOption (let open FStar.Getopt in noshort, "version", ZeroArgs (fun _ -> FStar.IO.print_string (Printf.sprintf "EverParse/3d %s\nCopyright 2018, 2019, 2020 Microsoft Corporation\n" Version.everparse_version); exit 0), "Show this version of EverParse");
+    CmdOption "equate_types" (OptList "an argument of the form A,B, to generate asserts of the form (A.t == B.t)" valid_equate_types equate_types_list) "Takes an argument of the form A,B and then for each entrypoint definition in B, it generates an assert (A.t == B.t) in the B.Types file, useful when refactoring specs, you can provide multiple equate_types on the command line" [];
+    CmdOption "__arg0" (OptString "executable name" always_valid arg0) "executable name to use for the help message" [];
+  ];
+  let fstar_options =
+    List.Tot.concatMap (fstar_options_of_cmd_option options) !options
+  in
+  (display_usage, fstar_options)
 
-let hidden_options =
-  let open FStar.Getopt in
-  [
-    (noshort, "__arg0", OneArg ((fun s -> arg0 := s), "executable name"), "executable name to use for the help message");
-  ]
+let display_usage = display_usage_2
 
 let parse_cmd_line () : ML (list string) =
   let open FStar.Getopt in
-  let res = FStar.Getopt.parse_cmdline (hidden_options `List.Tot.append` !options) (fun file -> input_file := file :: !input_file) in
+  let res = FStar.Getopt.parse_cmdline fstar_options (fun file -> input_file := file :: !input_file) in
   match res with
   | Success -> !input_file
   | Help -> display_usage(); exit 0
@@ -140,23 +333,13 @@ let split_3d_file_name fn =
 let get_file_name mname = mname ^ ".3d"
 
 let get_module_name (file: string) =
-  match !module_name with
-  | None ->
-    begin
     match split_3d_file_name file with
     | Some nm -> nm
     | None -> "DEFAULT"
-    end
-  | Some s ->
-    match !input_file with
-    | _ :: _ :: _ ->
-      failwith "module_name not allowed if several files are provided"
-    | _ -> s
 
 let get_output_dir () =
-  match !output_dir with
-  | None -> "."
-  | Some s -> s
+  let s = !output_dir in
+  if s = "" then "." else !output_dir
 
 let get_error_log () =
   match !error_log with
@@ -189,10 +372,15 @@ let get_skip_makefiles () =
   !skip_makefiles
 
 let get_no_everparse_h () =
-  !no_everparse_h
+  not !no_copy_everparse_h
 
 let get_check_hashes () =
-  if !batch then !check_hashes else None
+  if !batch then match !check_hashes with
+  | None -> None
+  | Some "weak" -> Some WeakHashes
+  | Some "strong" -> Some StrongHashes
+  | Some "inplace" -> Some InplaceHashes
+  else None
 
 let get_save_hashes () =
   !save_hashes
@@ -200,4 +388,9 @@ let get_save_hashes () =
 let get_check_inplace_hashes () =
   List.rev !inplace_hashes
 
-let get_equate_types_list () = !equate_types_list
+let get_equate_types_list () =
+  List.map
+    (fun (x: valid_string valid_equate_types) ->
+      let [a; b] = String.split [','] x in (a, b)
+    )
+    !equate_types_list
